Core/ProgramRules.v
@@ -7,10 +7,85 @@ From LHL.Core Require Import
   ProgramFacts.
 
 From Coq Require Import
-  Program.Equality.
+  Program.Equality
+  Logic.PropExtensionality.
 
 From LHL.Util Require Import
   Tactics.
+
+From Paco Require Import paco.
+
+Inductive paco_safeF {E F A} {VE : Spec E} {VF : Spec F} i (R G : Relt VE VF) (Q : Post VE VF A) (rec : Relt VE VF -> Prog E A -> Prop) : Relt VE VF -> Prog E A -> Prop :=
+| SafeReturn v P :
+    P ==> Q v ->
+    paco_safeF i R G Q rec P (Return v)
+| SafeBind A (P : Relt VE VF) QI QR (m : E A) k :
+    Stable R QI ->
+    Stable R QR ->
+    Commit i G P (CallEv m) QI ->
+    (forall v,
+      Commit i G (P ->> QI) (RetEv m v) (QR v) /\
+      rec (P ->> QI ->> QR v) (k v)) ->
+    paco_safeF i R G Q rec P (Bind m k)
+| SafeNoOp (P : Relt VE VF) QS C :
+    Stable R QS ->
+    SilentStep i G P QS ->
+    rec (P ->> QS) C ->
+    paco_safeF i R G Q rec P (NoOp C)
+.
+
+Definition paco_safe {E F A} {VE : Spec E} {VF : Spec F} i (R G P : Relt VE VF) (C : Prog E A) (Q : Post VE VF A) : Prop := paco2 (paco_safeF i R G Q) bot2 P C.
+
+Lemma safe_monotone {E F A} {VE : Spec E} {VF : Spec F} (i : ThreadName) (R G : Relt VE VF) (Q : Post VE VF A) :
+  monotone2 (paco_safeF i R G Q).
+unfold monotone2. intros.
+destruct IN.
+econstructor. easy.
+econstructor. exact H. exact H0. easy.
+intros. specialize (H2 v).
+split. easy.
+apply LE. easy.
+econstructor. exact H. easy.
+apply LE. easy.
+Qed.
+Hint Resolve safe_monotone : paco.
+
+CoFixpoint paco_eqv_help {E F A} {VE : Spec E} {VF : Spec F} (i : ThreadName) (R G : Relt VE VF) (Q : Post VE VF A) (P : Relt VE VF) (C : Prog E A):
+  paco_safe i R G P C Q -> SafeProg i R G P C Q.
+intros.
+punfold H.
+dependent destruction H.
+econstructor. easy.
+econstructor. exact H. exact H0. easy.
+intros. specialize (H2 v). destruct_all.
+split. easy.
+destruct H3.
+apply paco_eqv_help. easy.
+destruct H3.
+destruct H1.
+econstructor. exact H. easy.
+apply paco_eqv_help. easy.
+destruct H1.
+Qed.
+
+Lemma paco_eqv {E F A} {VE : Spec E} {VF : Spec F} (i : ThreadName) (R G : Relt VE VF) (Q : Post VE VF A) (P : Relt VE VF) (C : Prog E A):
+  SafeProg i R G P C Q = paco_safe i R G P C Q.
+apply propositional_extensionality.
+split; intros.
+{
+  generalize dependent C. generalize dependent P.
+  pcofix rec. intros. pfold.
+  destruct H0.
+  econstructor. easy.
+  econstructor. exact H. exact H0. easy.
+  intros. specialize (H2 v). destruct_all.
+  split. easy.
+  right. apply rec. easy.
+  econstructor. exact H. easy.
+  right. apply rec. easy.
+}
+apply paco_eqv_help. easy.
+Qed.
 
 Section rules.
 
@@ -60,83 +135,236 @@ econstructor. unfold sub, subRelt. intros.
 easy.
 Qed.
 
-Axiom undef:forall{a},a.
-
-CoFixpoint lemBind {A B P Q S} {C : Prog E A} {k : A -> Prog E B}
-  (H : VerifyProg i R G P C Q) :
+Lemma lemBind {A B P S} {C : Prog E A} {k : A -> Prog E B} :
+  forall Q,
+  VerifyProg i R G P C Q ->
   (forall v, VerifyProg i R G (Q v) (k v) S) ->
   VerifyProg i R G P (x <- C; k x) S.
+unfold VerifyProg.
 intros.
-destruct H.
+repeat rewrite paco_eqv in *.
+generalize dependent P. generalize dependent C. generalize dependent Q.
+generalize dependent k. generalize dependent A.
+pcofix rec. intros.
+punfold H1. dependent destruction H1.
 {
   rewrite frobProgId at 1. simpl.
-  assert (match k v with | @Bind _ _ A0 e f => Bind e f | Return a =>  Return a | NoOp p' => NoOp p' end = k v) by (destruct (k v); easy).
-  rewrite H1. clear H1.
-  eapply weakenSafe. exact H.
-  apply H0.
+  assert (k v = match k v with
+  | @Bind _ _ A0 e f => Bind e f
+  | Return a => Return a
+  | NoOp p' => NoOp p'
+  end) by (destruct (k v); easy). rewrite <- H1. clear H1.
+  specialize (H0 v).
+  rewrite paco_eqv in H0. punfold H0.
+  clear rec.
+  generalize dependent P. generalize dependent (Q v).
+  generalize dependent (k v). clear k v Q.
+  pcofix rec. intros.
+  pfold. dependent destruction H0.
+  {
+    econstructor.
+    unfold sub, subRelt in *.
+    auto.
+  }
+  {
+    econstructor.
+    exact H. exact H0.
+    eapply weakenCommitPre. exact H3. easy.
+    intros. specialize (H2 v). destruct_all.
+    split.
+    eapply weakenCommitPre with (P:= P ->> QI).
+    unfold sub, subRelt, ReltCompose. intros. destruct_all.
+    repeat eexists.
+    apply H3. exact H5. easy.
+    easy.
+    destruct H4.
+    punfold H4.
+    right. eapply rec. exact H4.
+    unfold sub, subRelt, ReltCompose. intros. destruct_all. repeat eexists.
+    apply H3. exact H5. exact H6. easy.
+    destruct H4.
+  }
+  {
+    destruct H1. 2: destruct H1.
+    econstructor. exact H.
+    unfold SilentStep. intros. apply H0.
+    unfold ReltToPrec in *. destruct_all. repeat eexists.
+    apply H2. exact H3.
+    easy. easy.
+    punfold H1.
+    right. eapply rec. exact H1.
+    unfold sub, subRelt, ReltCompose. intros. destruct_all. repeat eexists.
+    apply H2. exact H3. easy.
+  }
 }
-(* {
-  rewrite frobProgId at 1. simpl.
-  econstructor. exact H. exact H1. easy.
-  intros.
-  specialize (H3 v).
+{
+  rewrite frobProgId at 1. simpl. pfold. econstructor.
+  exact H. exact H1. easy.
+  intros. specialize (H3 v). destruct_all.
   split. easy.
-  destruct_all.
-  eapply lemBind.
-  exact H4.
-  exact H0.
-} *)
-apply undef.
-{
+  destruct H4. 2: destruct H4.
+  punfold H4.
+  right.
+  eapply rec. exact H0.
+  pfold. easy.
 }
-apply undef.
+{
+  rewrite frobProgId at 1. simpl. pfold. econstructor.
+  exact H. easy.
+  destruct H2. 2: destruct H2.
+  punfold H2. right.
+  eapply rec. exact H0.
+  pfold. easy.
+}
 Qed.
 
-Lemma weakenPost {A P Q Q'} {C : Prog E A} :
+
+Lemma weakenPost {A P} {C : Prog E A} :
+  forall Q Q',
   VerifyProg i R G P C Q ->
   (forall v, Q v ==> Q' v) ->
   VerifyProg i R G P C Q'.
-Admitted.
+unfold VerifyProg. intros.
+repeat rewrite paco_eqv in *.
+generalize dependent P. generalize dependent C.
+pcofix rec. intros.
+punfold H1. pfold.
+dependent destruction H1.
+{
+  econstructor. unfold sub, subRelt in *.
+  intros. apply H0. apply H. easy.
+}
+{
+  econstructor. exact H. exact H1. easy.
+  intros. specialize (H3 v). destruct_all.
+  split. easy.
+  destruct H4. 2: destruct H4.
+  right. eapply rec. easy.
+}
+{
+  destruct H2. 2: destruct H2.
+  econstructor. exact H. easy.
+  right. apply rec. easy.
+}
+Qed.
 
-Lemma weakenPrec {A P P' Q} {C : Prog E A} :
+Lemma weakenPrec {A Q} {C : Prog E A} :
+  forall P P',
   VerifyProg i R G P C Q ->
   P' ==> P ->
   VerifyProg i R G P' C Q.
-Admitted.
+intros.
+eapply weakenSafe.
+exact H0. easy.
+Qed.
 
-Lemma lemWhile {P} {T : Post VE VF bool} {Q : Post VE VF unit} {t : Prog E bool} {C : Prog E unit} :
-  (forall v, id ==> Q v) ->
-  P <<- T <<- Q ==> P ->
-  (forall v, (Q ->> T ->> Q v) ==> Q v) ->
-  VerifyProg i R G P t T ->
-  VerifyProg i R G (P <<- T) C Q ->
-  VerifyProg i R G P (while t C) (fun v => T ->> Q v).
-intros idQ subP inv safe_t safe_C.
-cofix rec.
-rewrite unfoldWhile.
-eapply lemBind.
-easy.
+Lemma foldProg {A} :
+  forall p : Prog E A,
+  match p with
+  | Return v => Return v
+  | Bind m k => Bind m k
+  | NoOp p => NoOp p
+  end = p.
 intros.
-destruct v.
-eapply weakenPost.
-eapply lemBind.
-exact safe_C.
+destruct p; easy.
+Qed.
+
+Definition SomeRet {A E F VE VF} (Q : @Post E F VE VF A) : Post VE VF unit :=
+  fun _ s ρ t σ => exists v, Q v s ρ t σ.
+
+Definition UnitRet {E F VE VF} (Q : @Relt E F VE VF) : Post VE VF unit :=
+  fun _ => Q.
+
+Lemma lemWhile {P} {T : Post VE VF bool} {B : Prog E bool} {C : Prog E unit} {S : Relt VE VF} :
+  Stable R S ->
+  SilentStep i G T S ->
+  T ->> S ==> P ->
+  VerifyProg i R G P B T ->
+  VerifyProg i R G (T true) C (SomeRet T) ->
+  VerifyProg i R G P (while B C) (UnitRet (T false)).
+unfold while, VerifyProg.
+intros S_stable S_step imp.
+repeat rewrite paco_eqv.
 intros.
-eapply weakenPrec.
-apply lemNoOp.
-exact rec.
-easy.
-intros.
-unfold sub, subRelt.
-intros.
-apply inv.
-easy.
-constructor.
-unfold sub, subRelt, id.
-intros.
-psimpl.
-apply idQ.
-easy.
+cut (
+  forall B' P',
+  paco_safe i R G P' B' T ->
+  paco_safe i R G P' (whileAux B C B' C) (UnitRet (T false))
+).
+{ intros. apply H1 with (P':=P). easy. }
+pcofix rec. intros. punfold H2. dependent destruction H2.
+{
+  destruct v.
+  2:{
+    pfold.
+    rewrite frobProgId at 1. cbn.
+    econstructor. easy.
+  }
+  rewrite <- paco_eqv in H0.
+  eapply weakenPrec with (P':=P0) in H0. 2: easy.
+  unfold VerifyProg in H0. rewrite paco_eqv in H0.
+  cut (
+    forall (P0' : Relt VE VF) C',
+    paco_safe i R G P0' C' (SomeRet T) ->
+    paco2 (paco_safeF i R G (UnitRet (T false))) r P0' (whileAux B C (Return true) C')
+  ).
+  {
+    intros. apply H2. easy.
+  }
+  pcofix rec'. intros. punfold H3. dependent destruction H3.
+  {
+    rewrite frobProgId at 1. cbn.
+    pfold. econstructor. exact S_stable.
+    {
+      unfold SilentStep. intros. apply S_step.
+      unfold ReltToPrec in *. destruct_all.
+      apply H2 in H3. destruct H3.
+      repeat eexists.
+      exact H3.
+      easy. easy.
+    }
+    {
+      right. eapply rec.
+      rewrite <- paco_eqv.
+      eapply weakenPrec with (P:=P).
+      unfold VerifyProg. rewrite paco_eqv.
+      easy.
+      unfold sub, subRelt. intros.
+      apply imp. psimpl.
+      apply H2 in H3. destruct H3.
+      repeat eexists. exact H3. easy.
+    }
+  }
+  {
+    rewrite frobProgId at 1. cbn. pfold. econstructor.
+    exact H2. exact H3. easy.
+    intros. specialize (H5 v). destruct_all.
+    split. easy.
+    destruct H6. 2: destruct H6.
+    right. eapply rec'. easy.
+  }
+  {
+    rewrite frobProgId at 1. cbn. pfold. econstructor.
+    exact H2. easy.
+    destruct H4. 2: destruct H4.
+    right. eapply rec'. easy.
+  }
+}
+{
+  pfold. rewrite frobProgId at 1. cbn.
+  econstructor. exact H1. exact H2. easy.
+  intros.
+  specialize (H4 v). destruct_all.
+  split. easy.
+  destruct H5. 2: destruct H5.
+  right. eapply rec. easy.
+}
+{
+  pfold. rewrite frobProgId at 1. cbn.
+  econstructor. exact H1. easy.
+  destruct H3. 2: destruct H3.
+  right. eapply rec. easy.
+}
 Qed.
 
 End rules.
